src/proof/controllers/replicaset/preservation.v
@@ -9,6 +9,18 @@ Collection W := sem + package_sem.
   code.controllers.replicaset.replicaset.import_common_Assumption.
 #[local] Instance controller_sem : controller.Assumptions :=
   code.controllers.replicaset.replicaset.import_controller_Assumption.
+#[local] Instance clientset_sem : kubernetes.Assumptions :=
+  code.controllers.replicaset.replicaset.import_kubernetes_Assumption.
+#[local] Instance client_core_v1_sem : client_core_v1.Assumptions :=
+  kubernetes.import_core_v1_Assumption.
+#[local] Instance client_apps_v1_sem : client_apps_v1.Assumptions :=
+  kubernetes.import_apps_v1_Assumption.
+#[local] Instance client_gentype_sem : client_gentype.Assumptions :=
+  client_core_v1.import_gentype_Assumption.
+#[local] Instance app_listers_sem : app_listers.Assumptions :=
+  code.controllers.replicaset.replicaset.import_listers_apps_v1_Assumption.
+#[local] Instance generic_listers_sem : generic_listers.Assumptions :=
+  app_listers.import_listers_Assumption.
 #[local] Instance runtime_sem : code.k8s_io.apimachinery.pkg.runtime.runtime.Assumptions :=
   controller.import_runtime_Assumption.
 #[local] Instance runtime_object_underlying_eq :
@@ -51,11 +63,28 @@ Proof.
   iDestruct "Hown_terminating_children_frag" as (phase) "Hown_terminating_children_frag".
   unfold input_requirement in Hinput_requirement.
   destruct Hinput_requirement as [Hrs_name_short Hrs_template_finalizers_valid].
-  wp_auto.
+  wp_pures.
+  wp_alloc_auto.
+  rewrite exception_do_unseal /exception_do_def.
+  wp_pures.
+  wp_alloc_auto. wp_pures.
+  wp_alloc_auto. wp_pures.
+  wp_alloc_auto. wp_pures.
+  wp_alloc_auto. wp_pures.
+  wp_alloc_auto. wp_pures.
+  wp_alloc_auto. wp_pures.
   iAssert (is_pkg_init common) as "#Hcommon_init".
   { iPkgInit. }
   iAssert (is_pkg_init apimodel) as "#Hapimodel".
   { iPkgInit. }
+  wp_load. wp_pure. wp_pure.
+  wp_load. wp_pure. wp_pure.
+  wp_load. wp_pure.
+  wp_bind (null @! (go.PointerType app_listers.replicaSetLister) @! "ReplicaSets" #namespace)%E.
+  wp_method_call. rewrite /trusted_app_listers.replicaSetLister__ReplicaSetsⁱᵐᵖˡ. wp_call. wp_auto.
+  wp_method_call. rewrite /trusted_generic_listers.ResourceIndexer__Getⁱᵐᵖˡ decide_True; try reflexivity.
+  rewrite /trusted_generic_listers.resourceIndexerGet. wp_pures.
+  wp_auto.
   wp_apply (wp_State__ReplicaSetGet with "[$Hown_rs_meta_frag $Hown_rs_spec_frag]").
   { iFrame "#".
     iPureIntro.
@@ -70,6 +99,8 @@ Proof.
     exact Hrs_get_spec_valid. }
   assert (ReplicaSetSpecV.valid rs.(ReplicaSetV.Spec')) as Hrs_spec_valid.
   { rewrite Hget_Hspec_eq. exact Hrs_get_spec_valid. }
+  wp_auto.
+  rewrite decide_True; try reflexivity.
   wp_auto.
   wp_apply (wp_IsNotFound interface.nil with "[]").
   replace (bool_decide (not_found_error interface.nil)) with false by
@@ -219,6 +250,7 @@ Proof.
       rs.(ReplicaSetV.ObjectMeta').(ObjectMetaV.UID') phase)%I
     with "[Hown_terminating_children_frag]" as "Hown_terminating_children_frag".
   { iExists phase'. iFrame. }
+  rewrite return_val_unseal /return_val_def. wp_auto.
   iApply ("HΦ" $! pods_managed).
   rewrite /owned_resources /=.
   iFrame "Hown_rs_meta_frag Hown_rs_spec_frag Hmanaged_meta_frags
