src/proof/k8s_io/client_go/applyconfigurations/autoscaling/v1_init.v
@@ -1,9 +1,5 @@
-From New.proof.k8s_io.api.apps Require Export v1_init.
-From New.proof.k8s_io.apimachinery.pkg Require Export labels_init.
-From New.proof.k8s_io.client_go Require Export listers_init.
-Require Export New.generatedproof.k8s_io.client_go.listers.apps.v1.
+Require Export New.generatedproof.k8s_io.client_go.applyconfigurations.autoscaling.v1.
 From New.proof Require Import proof_prelude.
-
 
 Section proof.
 Context `{hG: heapGS Σ} `{!ffi_semantics _ _}.
