src/trusted_code/k8s_io/client_go/listers.v
@@ -1,0 +1,59 @@
+From New.golang Require Import defn.
+Require Import New.code.kubernetes_model.apimodel.
+Require Import New.code.k8s_io.api.apps.v1.
+Require Import New.code.k8s_io.api.core.v1.
+Module api_apps_v1 := code.k8s_io.api.apps.v1.v1.
+Module api_core_v1 := code.k8s_io.api.core.v1.v1.
+
+Module listers.
+Section code.
+Context {ext : ffi_syntax} {go_gctx : GoGlobalContext}.
+
+(* Trusted Go equivalent:
+
+   func (l ResourceIndexer[T]) Get(name string) (T, error) {
+       var zero T
+       switch any(zero).(type) {
+       case *corev1.Pod:
+           obj, err := apimodel.ModelState.PodGet(l.namespace, name)
+           return any(obj).(T), err
+       case *appsv1.ReplicaSet:
+           obj, err := apimodel.ModelState.ReplicaSetGet(l.namespace, name)
+           return any(obj).(T), err
+       case *corev1.PersistentVolumeClaim:
+           obj, err := apimodel.ModelState.PersistentVolumeClaimGet(l.namespace, name)
+           return any(obj).(T), err
+       case *appsv1.StatefulSet:
+           obj, err := apimodel.ModelState.StatefulSetGet(l.namespace, name)
+           return any(obj).(T), err
+       default:
+           panic("unsupported Kubernetes object type")
+       }
+   }
+*)
+Definition resourceIndexerGet (T : go.type) (method : go_string) : val :=
+  λ: "namespace" "name",
+    (* The trusted lister constructor represents its ResourceIndexer by the
+       namespace string, which is the only receiver state used by this shim. *)
+    let: "namespace" := (GoAlloc go.string "namespace") in
+    let: "name" := (GoAlloc go.string "name") in
+    let: ("$ret0", "$ret1") := (let: "$a0" := (![go.string] "namespace") in
+    let: "$a1" := (![go.string] "name") in
+    (MethodResolve (go.PointerType apimodel.State) method
+      (![go.PointerType apimodel.State] (GlobalVarAddr apimodel.ModelState #()))) "$a0" "$a1") in
+    (TypeAssert T (Convert T go.any "$ret0"), "$ret1").
+
+Definition ResourceIndexer__Getⁱᵐᵖˡ (T : go.type) : val :=
+  if decide (T = go.PointerType api_apps_v1.ReplicaSet) then
+    resourceIndexerGet T "ReplicaSetGet"%go
+  else if decide (T = go.PointerType api_core_v1.Pod) then
+    resourceIndexerGet T "PodGet"%go
+  else if decide (T = go.PointerType api_core_v1.PersistentVolumeClaim) then
+    resourceIndexerGet T "PersistentVolumeClaimGet"%go
+  else if decide (T = go.PointerType api_apps_v1.StatefulSet) then
+    resourceIndexerGet T "StatefulSetGet"%go
+  else
+    (λ: "namespace" "name", Panic "unsupported Kubernetes object type")%V.
+
+End code.
+End listers.
