src/code/k8s_io/client_go/gentype.v
@@ -411,6 +411,7 @@ Class Client_Assumptions {ext : ffi_syntax} `{!GoGlobalContext} `{!GoLocalContex
   #[global] Client_set_prefersProtobuf T T' (x : Client.t T') y :: ⟦StructFieldSet (Clientⁱᵐᵖˡ T) "prefersProtobuf", (#x, #y)⟧ ⤳[under] #(x <|Client.prefersProtobuf' := y|>);
   #[global] Client'ptr_Create_unfold T :: MethodUnfold (go.PointerType (Client T)) "Create" (Client__Createⁱᵐᵖˡ T);
   #[global] Client'ptr_Delete_unfold T :: MethodUnfold (go.PointerType (Client T)) "Delete" (Client__Deleteⁱᵐᵖˡ T);
+  #[global] Client'ptr_Get_unfold T :: MethodUnfold (go.PointerType (Client T)) "Get" (Client__Getⁱᵐᵖˡ T);
 }.
 
 Module alsoLister.
